Labelled Gentzen, soundness

ModalTableau/Basic.lean
@@ -1,210 +1,66 @@
 import Foundation.Modal.NNFormula
+import Foundation.Modal.Kripke.Basic
 
 namespace LO.Modal
 
-open NNFormula
 
-namespace Tableau
+namespace Labelled
+
+
+abbrev Label := ℕ
+
+namespace Label
+
+def Assignment (M : Kripke.Model) := Label → M.World
+
+end Label
+
+
+abbrev LabelTerm := Label × Label
+
+namespace LabelTerm
+
+def evaluated {M : Kripke.Model} (f : Label.Assignment M) : LabelTerm → Prop := λ ⟨x, y⟩ => M.Rel (f x) (f y)
+
+end LabelTerm
 
 
 structure LabelledFormula where
-  label : ℕ
-  formula : NNFormula ℕ
+  label : Label
+  formula : Formula ℕ
+deriving DecidableEq, Repr
 
 namespace LabelledFormula
 
-notation:max l " ∶ " φ => LabelledFormula.mk l φ
+notation:95 x " ∶ " φ => LabelledFormula.mk x φ
 
-section toStr
+def Satisfies (M : Kripke.Model) (f : Label.Assignment M) : LabelledFormula → Prop := λ (x ∶ φ) => (f x) ⊧ φ
 
-def toStr (lf : LabelledFormula) : String := s!"{lf.label} : {lf.formula.toStr}"
+namespace Satisfies
 
-instance : Repr (LabelledFormula) := ⟨λ t _ => toStr t⟩
-instance : ToString (LabelledFormula) := ⟨toStr⟩
-
-#eval (0 ∶ (atom 1 ➝ atom 2))
-
-end toStr
+protected instance semantics {M : Kripke.Model} : Semantics (LabelledFormula) (Label.Assignment M) := ⟨fun x ↦ LabelledFormula.Satisfies M x⟩
 
 
-section deq
+variable {M : Kripke.Model} {f : Label.Assignment M}
+variable {x y : Label}
+variable {φ ψ : Formula ℕ} {xφ: LabelledFormula}
 
-def deq (lf₁ lf₂ : LabelledFormula) : Bool := lf₁.formula = lf₂.formula
-instance : BEq LabelledFormula := ⟨deq⟩
+@[simp] protected lemma iff_models : f ⊧ (x ∶ φ) ↔ f x ⊧ φ := by tauto;
 
-end deq
+lemma imp_def : f ⊧ (x ∶ φ ➝ ψ) ↔ (f x) ⊧ φ ➝ ψ := by tauto;
 
+lemma box_def : f ⊧ (x ∶ □φ) ↔ (f x) ⊧ □φ := by tauto;
+
+end Satisfies
 
 end LabelledFormula
 
 
+structure LabelledNNFormula where
+  label : Label
+  formula : NNFormula ℕ
+deriving DecidableEq, Repr
 
-abbrev RelTerm := ℕ × ℕ
-
-namespace RelTerm
-
-notation a " ≺ " b => (a, b)
-
-section toStr
-
-def toStr (rt : RelTerm) : String := s!"{rt.1} ≺ {rt.2}"
-instance : Repr RelTerm := ⟨λ t _ => toStr t⟩
-instance : ToString RelTerm := ⟨toStr⟩
-
-end toStr
-
-end RelTerm
-
-
-
-abbrev RelTerms := List RelTerm
-
-namespace RelTerms
-
-abbrev rel (rs : RelTerms) := rs.contains
-
-end RelTerms
-
-
-structure GenFormula where
-  formula : LabelledFormula
-  generated : List LabelledFormula
-deriving Repr, BEq
-
-
-structure Path where
-  path : List GenFormula
-  rels : List (ℕ × ℕ)
-deriving Repr
-
-namespace Path
-
-section toStr
-
--- def toStr (P : Path) : String := P.map (λ ⟨lφ, g⟩ => s!"{lφ} => {g}\n") |> String.join
-
--- instance : Repr Path := ⟨λ t _ => toStr t⟩
-
-#eval (⟨[
-    ⟨(0 ∶ atom 1), []⟩,
-    ⟨(0 ∶ atom 1 ⋏ atom 2), []⟩
-  ], []⟩ : Path)
-
-def insert_gf (gf : GenFormula) : Path → Path := λ ⟨path, rels⟩ => ⟨path.insert gf, rels⟩
-
-end toStr
-
-partial def applyRules₁ : Path → List (Path) := λ ⟨nodes, rels⟩ =>
-  match nodes with
-  | [] => [⟨[], rels⟩]
-  | ⟨l ∶ atom p, []⟩ :: rest =>
-    applyRules₁ ⟨rest, rels⟩ |>.map $ insert_gf ⟨l ∶ atom p, [l ∶ atom p]⟩
-  | ⟨l ∶ natom p, []⟩ :: rest =>
-    applyRules₁ ⟨rest, rels⟩ |>.map $ insert_gf ⟨l ∶ natom p, [l ∶ natom p]⟩
-  | ⟨l ∶ φ ⋏ ψ, []⟩ :: rest =>
-    applyRules₁ (⟨rest |>.insert ⟨l ∶ ψ, []⟩ |>.insert ⟨l ∶ φ, []⟩, rels⟩) |>.map $ insert_gf ⟨l ∶ φ ⋏ ψ, [l ∶ φ, l ∶ ψ]⟩
-  | ⟨l ∶ φ ⋎ ψ, []⟩ :: rest =>
-    (applyRules₁ ⟨rest.insert ⟨l ∶ φ, []⟩, rels⟩ |>.map $ insert_gf ⟨l ∶ φ ⋎ ψ, [l ∶ φ]⟩)
-    ++
-    (applyRules₁ ⟨rest.insert ⟨l ∶ ψ, []⟩, rels⟩ |>.map $ insert_gf ⟨l ∶ φ ⋎ ψ, [l ∶ ψ]⟩)
-  | ⟨l ∶ ◇φ, []⟩ :: rest =>
-    letI m := (l :: rest.map (λ ⟨⟨l, _⟩, _⟩ => l) ++ (rels.map (λ ⟨x, y⟩ => [x, y]) |>.flatten) |>.foldl max 0) + 1
-    applyRules₁ ⟨rest.insert ⟨m ∶ φ, []⟩, rels.insert (l, m)⟩ |>.map $ insert_gf ⟨l ∶ ◇φ, [m ∶ φ]⟩
-  | gφ :: rest =>
-    applyRules₁ ⟨rest, rels⟩ |>.map $ insert_gf gφ
-
-#eval applyRules₁ ⟨[
-    ⟨0 ∶ ∼(□(atom 0 ➝ atom 1) ➝ □(atom 0) ➝ □(atom 1)), []⟩,
-  ], []⟩
-
-#eval applyRules₁ ⟨[
-    ⟨0 ∶ natom 1 ⋏ (atom 2 ⋏ atom 3), []⟩,
-    ⟨0 ∶ atom 4 ⋏ atom 5, []⟩,
-    ⟨0 ∶ atom 1, []⟩,
-  ], []⟩
-
-
-#eval applyRules₁ ⟨[
-    ⟨0 ∶ atom 1 ⋎ (atom 2 ⋏ atom 3), []⟩,
-    ⟨0 ∶ atom 4 ⋏ atom 5, []⟩,
-    ⟨0 ∶ atom 1, []⟩,
-  ], []⟩
-
-#eval applyRules₁ ⟨[
-    ⟨0 ∶ ◇(atom 0 ⋏ natom 1), []⟩,
-  ], []⟩
-
-#eval applyRules₁ ⟨[
-    ⟨0 ∶ ◇(atom 1), []⟩,
-    ⟨1 ∶ ◇(atom 0 ⋏ ◇(natom 1)), []⟩,
-    ⟨2 ∶ ◇(atom 2), []⟩,
-  ], []⟩
-
-#eval (applyRules₁ ⟨[
-    ⟨0 ∶ ◇◇◇(atom 1 ⋏ □(atom 2)), []⟩,
-    ⟨0 ∶ ◇◇◇(atom 3 ⋏ □(atom 4)), []⟩,
-  ], []⟩)
-
-
-partial def applyRules₂ : Path → Path := λ ⟨nodes, rels⟩ =>
-  match nodes with
-  | [] => ⟨[], rels⟩
-  | ⟨l ∶ □φ, c⟩ :: rest =>
-    letI tos : List LabelledFormula := rels
-      |>.filter (λ ⟨f, _⟩ => f = l)
-      |>.map (λ ⟨_, t⟩ => t ∶ φ)
-      |>.filter (!c.contains ·)
-    let ges : List GenFormula := tos.map (λ t => ⟨t, []⟩)
-    applyRules₂ (⟨rest ++ ges, rels⟩) |>.insert_gf ⟨l ∶ □φ, c ++ tos⟩
-    -- Path.insert_gf ⟨l ∶ □φ, c ++ tos⟩ (⟨rest ++ ps, rels⟩)
-  | gφ :: rest =>
-    applyRules₂ ⟨rest, rels⟩ |>.insert_gf gφ
-
-#eval (applyRules₂ ⟨[
-    ⟨0 ∶ □(atom 1 ⋏ □(atom 2)), []⟩,
-  ], [(0, 1), (0, 2)]⟩)
-
-#eval (applyRules₂ ⟨[
-    ⟨0 ∶ □(atom 1 ⋏ □(atom 2)), []⟩,
-  ], [(0, 1), (0, 2), (0, 3), (2, 0)]⟩)
-
-#eval (applyRules₁ $ applyRules₂ ⟨[
-    ⟨0 ∶ □(atom 1 ⋏ □(natom 2)), []⟩,
-  ], [(0, 1), (0, 2), (0, 3), (2, 0)]⟩) |>.map applyRules₂
-
-#eval (applyRules₂ ⟨[
-    ⟨0 ∶ □(atom 0), []⟩,
-    ⟨2 ∶ □(atom 1 ⋏ □(natom 2)), []⟩,
-  ], [(2, 0), (0, 2), (0, 1)]⟩)
-
-#eval (applyRules₁ $ (applyRules₂ ⟨[
-    ⟨0 ∶ □(atom 0), []⟩,
-    ⟨2 ∶ □(atom 1 ⋏ □(natom 2)), []⟩,
-  ], [(2, 0), (0, 2), (0, 1)]⟩)) |>.map applyRules₂
-
-#eval (⟨[
-    ⟨0 ∶ ∼(□(atom 0 ➝ atom 1) ➝ □(atom 0) ➝ □(atom 1)), []⟩,
-  ], []⟩ : Path) |>.applyRules₁ |>.map applyRules₂ |> (List.map applyRules₁)
-
-abbrev applyRules := List.flatten ∘ (List.map (applyRules₁ ∘ applyRules₂))
-
-
-#eval applyRules $ applyRules $ applyRules $ applyRules [(⟨[
-    ⟨0 ∶ ∼(□(atom 0 ➝ atom 1) ➝ □(atom 0) ➝ □(atom 1)), []⟩,
-  ], []⟩ : Path)]
-
-
-def isClosed (P : Path) : Bool :=
-  let lφs := P.path.map (λ ⟨lφ, _⟩ => lφ)
-  lφs.any (λ ⟨l, φ⟩ => lφs.contains ⟨l, ∼φ⟩)
-
-#eval applyRules [(⟨[⟨0 ∶ ∼(□(atom 0 ➝ atom 1) ➝ □(atom 0) ➝ □(atom 1)), []⟩], []⟩ : Path)]
-    |>.map (λ P => P.isClosed)
-
-end Path
-
-
-
-end Tableau
+end Labelled
 
 end LO.Modal
